experiments/SmallStepExperiment.v
@@ -5,6 +5,7 @@ From ITree Require Import
 From Paco Require Import paco.
 
 Require Import ProofIrrelevance.
+Require Import Classical_Prop.
 
 Require Import List.
 Import ListNotations.
@@ -126,6 +127,11 @@ Proof.
   -
 Admitted.
 
+Ltac invert_existTs :=
+  repeat match goal with
+         | [ H : existT ?P ?p _ = existT ?P ?p _ |- _ ] => apply inj_pair2 in H
+         end.
+
 Lemma is_trace_unalltaus: forall {E R} (t t' : itree E R) l r n,
     is_trace t l r ->
     unalltaus n t t' ->
@@ -135,6 +141,7 @@ Proof.
   - constructor.
   - rewrite (itree_eta t') in *. destruct (observe t'); inversion H0; subst; constructor.
   - eapply IHis_trace. apply (unalltaus_tau _ _ _ H0).
+  - inversion H0; subst; clear H0. constructor. auto.
   - inversion H0; subst; clear H0. constructor. auto.
 Qed.
 
@@ -152,6 +159,15 @@ Lemma euttF_tau_one {E R} r (t1 t2 : itree E R) :
 Proof.
   intros. destruct H. econstructor.
   - rewrite <- finite_taus_tau. eauto.
+  - intros. eapply EQV; apply unalltaus_tau; eauto.
+Qed.
+
+Lemma euttF_tau_one' {E R} r (t1 t2 : itree E R) :
+  (euttF r t1 (Tau t2)) ->
+  euttF r t1 t2.
+Proof.
+  intros. destruct H. econstructor.
+  - symmetry. rewrite <- finite_taus_tau. symmetry. eauto.
   - intros. eapply EQV; apply unalltaus_tau; eauto.
 Qed.
 
@@ -179,7 +195,7 @@ Proof.
     assert (unalltaus 0 (Vis e k) (Vis e k)) by auto.
     pinversion H. pose proof (EQV _ x0 (Vis e k) x1 H2 H1) as EQV'. inversion EQV'. clear EQV'.
 
-    apply inj_pair2 in H5. apply inj_pair2 in H6. subst.
+    invert_existTs. subst.
 
     remember (Vis _ _) in H1.
     induction H1; subst; constructor.
@@ -187,6 +203,18 @@ Proof.
     * apply IHuntaus; auto. constructor.
         - rewrite finite_taus_tau in FIN. auto.
         - intros. eapply EQV; apply unalltaus_tau; eauto.
+        - rewrite finite_taus_tau in FIN. auto.
+        - intros. eapply EQV; apply unalltaus_tau; eauto.
+  + assert (FINt2: finite_taus t2).
+    { apply (finite_taus_eutt _ _ H0). apply notau_finite_taus; auto. }
+    destruct FINt2. destruct H1.
+
+    assert (unalltaus 0 (Vis e k) (Vis e k)) by auto.
+    pinversion H0. pose proof (EQV _ x (Vis e k) x0 H2 H1) as EQV'. inversion EQV'. clear EQV'.
+    invert_existTs; subst.
+    remember (Vis _ _) in H1. induction H1; subst; constructor; auto.
+    apply IHuntaus; auto.
+        - apply euttF_tau_one'. auto.
         - rewrite finite_taus_tau in FIN. auto.
         - intros. eapply EQV; apply unalltaus_tau; eauto.
 Qed.
@@ -226,7 +254,7 @@ Proof.
         symmetry. apply is_trace_tau_iff. symmetry. apply H.
       * apply finite_taus_vis.
     + inversion PROP.
-    + assert (inhabited u \/ ~inhabited u) by admit. destruct H0.
+    + destruct (classic (inhabited u)).
       {
         inversion H0.
         assert (is_trace (Vis e k) [Event e X] None) by repeat constructor.
@@ -237,13 +265,18 @@ Proof.
         - apply finite_taus_vis.
       }
       {
-        assert (is_trace (Vis e k) [] None) by constructor.
-        rewrite H in H1. admit.
+        assert (is_trace (Vis e k) [OutputEvent e] None) by (constructor; auto).
+        rewrite H in H1.
+
+        remember [OutputEvent e] as l in H1. induction H1; try solve [inversion Heql]; subst.
+        - rewrite finite_taus_tau. apply IHis_trace; auto. intros.
+          symmetry. apply is_trace_tau_iff. symmetry. apply H.
+        - apply finite_taus_vis.
       }
       (* assert (is_trace (Vis e k) [] None) by constructor. *)
       (* rewrite H in H0. *)
   - apply IHuntaus. intros. apply is_trace_tau_iff. auto.
-Admitted.
+Qed.
 
 Lemma eutt_traces: forall {E R} (t1 t2 : itree E R),
     eutt t1 t2 ->
@@ -254,7 +287,65 @@ Proof.
   - apply Symmetric_eutt in H. apply (eutt_is_trace _ _ _ _ H H0).
 Qed.
 
-(* TODO clean up this counterexample *)
+Lemma unalltaus_tau_false: forall {E R} n (t t' : itree E R), unalltaus n t (Tau t') -> False.
+Proof.
+  intros. remember (Tau t') as t''. induction H; subst; auto.
+Qed.
+
+
+Lemma traces_eutt: forall {E R} (t1 t2 : itree E R),
+    (forall t r, is_trace t1 t r <-> is_trace t2 t r) ->
+    eutt t1 t2.
+Proof.
+  intros E R.
+  pcofix CIH. intros t1 t2 Hiff. pfold. constructor.
+  - split.
+    + apply traces_equiv_finite_taus; auto.
+    + symmetry in Hiff. apply traces_equiv_finite_taus; auto.
+  - intros. assert (Hiff': forall t r, is_trace t1' t r <-> is_trace t2' t r).
+    { intros. split; intros.
+      - pose proof (is_trace_unalltaus' _ _ _ _ _ H UNTAUS1).
+        rewrite Hiff in H0. eapply is_trace_unalltaus; eauto.
+      - pose proof (is_trace_unalltaus' _ _ _ _ _ H UNTAUS2).
+        rewrite <- Hiff in H0. eapply is_trace_unalltaus; eauto.
+    }
+    rewrite (itree_eta t1') in *. rewrite (itree_eta t2') in *.
+    destruct (observe t1') in *; destruct (observe t2');
+      try solve [contradiction (unalltaus_tau_false _ _ _ UNTAUS1)];
+      try solve [contradiction (unalltaus_tau_false _ _ _ UNTAUS2)].
+    + assert (is_trace (Ret r0 : itree E R) [] (Some r0)) by constructor.
+      rewrite Hiff' in H. inversion H; subst. constructor.
+    + assert (is_trace (Ret r0 : itree E R) [] (Some r0)) by constructor.
+      rewrite Hiff' in H. inversion H.
+    + assert (is_trace (Ret r0 : itree E R) [] (Some r0)) by constructor.
+      rewrite <- Hiff' in H. inversion H.
+    + destruct (classic (inhabited u)).
+      * destruct H. assert (is_trace (Vis e k) [Event e X] None) by (repeat constructor).
+        rewrite Hiff' in H. inversion H; subst. invert_existTs; subst.
+        constructor.
+        intros. right. apply CIH. intros. split; intros.
+        { assert (is_trace (Vis e k) ((Event e x) :: t) r0) by (constructor; auto).
+          rewrite Hiff' in H1. inversion H1; auto. invert_existTs; subst; auto.
+        }
+        { assert (is_trace (Vis e k0) ((Event e x) :: t) r0) by (constructor; auto).
+          rewrite <- Hiff' in H1. inversion H1; auto. invert_existTs; subst; auto.
+        }
+      * assert (is_trace (Vis e k) [OutputEvent e] None) by (constructor; auto).
+        rewrite Hiff' in H0. inversion H0; subst. invert_existTs; subst.
+        constructor. intros. exfalso. apply H.
+        apply exists_inhabited with (P:=fun x => True). exists x. auto.
+Qed.
+
+Lemma final: forall {E R} (t1 t2 : itree E R),
+    t1 ~~ t2 <->
+    (forall t r, is_trace t1 t r <-> is_trace t2 t r).
+Proof.
+  intros. split; intro.
+  - apply eutt_traces; auto.
+  - apply traces_eutt; auto.
+Qed.
+
+(* counterexample for old defn of is_trace *)
 Lemma is_trace_but_not_eutt : forall {E R} (X : Type) (e : E X) (k : X -> itree E R),
     (~inhabited X) ->
     (forall t r, is_trace ITree.spin t r <-> is_trace (Vis e k) t r)
@@ -266,58 +357,10 @@ Proof.
     + unfold ITree.spin in Heqtree. rewrite itree_eta in Heqtree. inversion Heqtree.
     + apply IHis_trace. rewrite itree_eta in Heqtree. inversion Heqtree. reflexivity.
     + unfold ITree.spin in Heqtree. rewrite itree_eta in Heqtree. inversion Heqtree.
+    + (* this last case does not exist for old defn of traces *)
+        unfold ITree.spin in Heqtree. rewrite itree_eta in Heqtree. inversion Heqtree.
   - remember (Vis e k) as tree. induction H0; try inversion Heqtree; subst.
     + constructor.
     + exfalso. apply H. apply exists_inhabited with (P:=fun _ => True). exists x. auto.
-Qed.
-
-(* Lemma is_trace_and_eutt : forall {E R} (X : Type) (e : E X) (k : X -> itree E R), *)
-(*     (inhabited X) -> *)
-(*     (forall t r, is_trace ITree.spin t r <-> is_trace (Vis e k) t r) *)
-(* . *)
-(* Proof. *)
-(*   intros. split; intro. *)
-(*   - remember ITree.spin as tree. induction H0. *)
-(*     + constructor. *)
-(*     + unfold ITree.spin in Heqtree. rewrite itree_eta in Heqtree. inversion Heqtree. *)
-(*     + apply IHis_trace. rewrite itree_eta in Heqtree. inversion Heqtree. reflexivity. *)
-(*     + unfold ITree.spin in Heqtree. rewrite itree_eta in Heqtree. inversion Heqtree. *)
-(*   - remember (Vis e k) as tree. induction H0; try inversion Heqtree; subst. *)
-(*     + constructor. *)
-(*     + exfalso. apply H. apply exists_inhabited with (P:=fun _ => True). exists x. auto. *)
-(* Qed. *)
-
-Lemma traces_eutt_false: ~ forall {E R} (t1 t2 : itree E R),
-                           (forall t r, is_trace t1 t r <-> is_trace t2 t r) -> eutt t1 t2.
-Proof.
-  intro.
-  Inductive Void : Type := .
-  Inductive E' : Type -> Type := | E'1 : forall x : Type, E' x.
-  specialize (H E' nat (Vis (E'1 Void) (fun _ => Ret 0)) (Vis (E'1 Void) (fun _ => Ret 1))).
-  assert ((Vis (E'1 Void) (fun _ => Ret 0)) ~~ (Vis (E'1 Void) (fun _ => Ret 1)) -> False). {
-    intro.
-    assert (unalltaus 0 (Vis (E'1 Void) (fun _ => Ret 0)) (Vis (E'1 Void) (fun _ => Ret 0))) by auto.
-    assert (unalltaus 0 (Vis (E'1 Void) (fun _ => Ret 1)) (Vis (E'1 Void) (fun _ => Ret 1))) by auto.
-    pinversion H0.
-    specialize (EQV 0 0 (Vis (E'1 Void) (fun _ => Ret 0)) (Vis (E'1 Void) (fun _ => Ret 1)) H1 H2).
-    inversion EQV.
-    apply inj_pair2 in H5. apply inj_pair2 in H6.
-    apply inj_pair2 in H7. apply inj_pair2 in H8. subst.
-  }
-  apply H0. apply H. intro.
-Qed.
-(*   { pcofix IH. pfold. constructor; intros. *)
-(*     - split; intros. *)
-(*       + eapply traces_equiv_finite_taus; eauto. *)
-(*       + symmetry in H. eapply traces_equiv_finite_taus; eauto. *)
-(*     - assert (forall t r, is_trace t1' t r <-> is_trace t2' t r). *)
-(*       { intros. split; intros. *)
-(*         - pose proof (is_trace_unalltaus' _ _ _ _ _ H0 UNTAUS1). *)
-(*           rewrite H in H1. eapply is_trace_unalltaus; eauto. *)
-(*         - pose proof (is_trace_unalltaus' _ _ _ _ _ H0 UNTAUS2). *)
-(*           rewrite <- H in H1. eapply is_trace_unalltaus; eauto. *)
-(*       } *)
-
-(*       rewrite (itree_eta t1'). rewrite (itree_eta t2') in *. destruct (observe t1') in *; destruct (observe t2'). *)
-(*       admit. *)
-(* Admitted. *)
+    + invert_existTs; subst.
+Abort.
